feat: basic compatibility lemma

CollapsingTowers/TwoLevelMut/LogicalEquiv/LogicalRelation.lean
@@ -45,21 +45,21 @@ def log_equiv_value : World → Expr → Expr → Ty → Prop
 -- 𝓔⟦τ⟧ ≜ {
 --   (𝓦₀, e₀, e₁) |
 --   ∀ (σ₀, σ₁) : 𝓦₀.
---   ∃ ω₀, ω₁, v₀, v₁, (𝓦₁ ⊒ 𝓦₀).
---     ⟨σ₀, e₀⟩ ⇝* ⟨ω₀, v₀⟩ ∧
---     ⟨σ₁, e₁⟩ ⇝* ⟨ω₁, v₁⟩ ∧
---     (ω₀, ω₁) : 𝓦₁ ∧
+--   ∃ σ₂, σ₃, v₀, v₁, (𝓦₁ ⊒ 𝓦₀).
+--     ⟨σ₀, e₀⟩ ⇝* ⟨σ₂, v₀⟩ ∧
+--     ⟨σ₁, e₁⟩ ⇝* ⟨σ₃, v₁⟩ ∧
+--     (σ₂, σ₃) : 𝓦₁ ∧
 --     (𝓦₁, v₀, v₁) ∈ 𝓥⟦τ⟧
 -- }
 @[simp]
 def log_equiv_expr (𝓦₀ : World) (e₀ e₁ : Expr) (τ : Ty) : Prop :=
   ∀ σ₀ σ₁,
     log_equiv_store 𝓦₀ σ₀ σ₁ →
-    ∃ 𝓦₁ ω₀ ω₁ v₀ v₁,
+    ∃ 𝓦₁ σ₂ σ₃ v₀ v₁,
       (𝓦₁ ⊒ 𝓦₀) ∧
-      (⟨σ₀, e₀⟩ ⇝* ⟨ω₀, v₀⟩) ∧
-      (⟨σ₁, e₁⟩ ⇝* ⟨ω₁, v₁⟩) ∧
-      log_equiv_store 𝓦₁ ω₀ ω₁ ∧
+      (⟨σ₀, e₀⟩ ⇝* ⟨σ₂, v₀⟩) ∧
+      (⟨σ₁, e₁⟩ ⇝* ⟨σ₃, v₁⟩) ∧
+      log_equiv_store 𝓦₁ σ₂ σ₃ ∧
       log_equiv_value 𝓦₁ v₀ v₁ τ
 end
 
@@ -141,3 +141,136 @@ lemma log_equiv_env.antimono :
     apply log_equiv_env.cons
     apply log_equiv_value.antimono; apply Hsem_value; apply Hfuture₀
     apply IH
+
+lemma log_equiv_value.syntactic.value :
+  ∀ 𝓦 v₀ v₁ τ,
+    log_equiv_value 𝓦 v₀ v₁ τ →
+    value v₀ ∧ value v₁ :=
+  by
+  intros 𝓦 v₀ v₁ τ Hsem_value
+  cases τ
+  case nat =>
+    cases v₀ <;> try simp at Hsem_value
+    case lit n₀ =>
+    cases v₁ <;> try simp at Hsem_value
+    case lit n₁ =>
+    constructor
+    apply value.lit
+    apply value.lit
+  case arrow τ𝕒 τ𝕓 φ =>
+    cases v₀ <;> try simp at Hsem_value
+    case lam e₀ =>
+    cases v₁ <;> try simp at Hsem_value
+    case lam e₁ =>
+    cases φ <;> simp only [log_equiv_value] at Hsem_value <;> try contradiction
+    have ⟨Hwf₀, HG₀, Hwf₁, HG₁, Hsem_value⟩ := Hsem_value
+    constructor
+    apply value.lam; apply Hwf₀.left
+    apply value.lam; apply Hwf₁.left
+  case unit =>
+    cases v₀ <;> try simp at Hsem_value
+    case unit =>
+    cases v₁ <;> try simp at Hsem_value
+    case unit =>
+    constructor
+    apply value.unit
+    apply value.unit
+  case ref τ =>
+    cases v₀ <;> try simp at Hsem_value
+    case loc l₀ =>
+    cases v₁ <;> try simp at Hsem_value
+    case loc l₁ =>
+    cases τ <;> simp only [log_equiv_value] at Hsem_value <;> try contradiction
+    constructor
+    apply value.loc
+    apply value.loc
+  case fragment => simp at Hsem_value
+  case rep => simp at Hsem_value
+
+lemma log_equiv_value.syntactic.wf :
+  ∀ k v₀ v₁ τ,
+    log_equiv_value k v₀ v₁ τ →
+    wf v₀ ∧ wf v₁ :=
+  by
+  intros 𝓦 v₀ v₁ τ Hsem_value
+  cases τ
+  case nat =>
+    cases v₀ <;> try simp at Hsem_value
+    case lit n₀ =>
+    cases v₁ <;> try simp at Hsem_value
+    case lit n₁ =>
+    simp
+  case arrow τ𝕒 τ𝕓 φ =>
+    cases v₀ <;> try simp at Hsem_value
+    case lam e₀ =>
+    cases v₁ <;> try simp at Hsem_value
+    case lam e₁ =>
+    cases φ <;> simp only [log_equiv_value] at Hsem_value <;> try contradiction
+    have ⟨Hwf₀, HG₀, Hwf₁, HG₁, Hsem_value⟩ := Hsem_value
+    constructor
+    apply Hwf₀
+    apply Hwf₁
+  case unit =>
+    cases v₀ <;> try simp at Hsem_value
+    case unit =>
+    cases v₁ <;> try simp at Hsem_value
+    case unit =>
+    simp
+  case ref τ =>
+    cases v₀ <;> try simp at Hsem_value
+    case loc l₀ =>
+    cases v₁ <;> try simp at Hsem_value
+    case loc l₁ =>
+    cases τ <;> simp only [log_equiv_value] at Hsem_value <;> try contradiction
+    simp
+  case fragment => simp at Hsem_value
+  case rep => simp at Hsem_value
+
+lemma log_equiv_value.apply :
+  ∀ 𝓦 f₀ arg₀ f₁ arg₁ τ𝕒 τ𝕓,
+    log_equiv_value 𝓦 f₀ f₁ (.arrow τ𝕒 τ𝕓 ⊥) →
+    log_equiv_value 𝓦 arg₀ arg₁ τ𝕒 →
+    log_equiv_expr 𝓦 (.app₁ f₀ arg₀) (.app₁ f₁ arg₁) τ𝕓 :=
+  by
+  intros 𝓦 f₀ arg₀ f₁ arg₁ τ𝕒 τ𝕓 Hsem_value_fun Hsem_value_arg
+  cases f₀ <;> cases f₁ <;> simp only [log_equiv_value] at Hsem_value_fun <;> try contradiction
+  have ⟨_, _, _, _, Hsem_value_fun⟩ := Hsem_value_fun
+  apply Hsem_value_fun; apply World.future.refl; apply Hsem_value_arg
+
+lemma log_equiv_env.length :
+  ∀ 𝓦 γ₀ γ₁ Γ,
+    log_equiv_env 𝓦 γ₀ γ₁ Γ →
+    γ₀.length = Γ.length ∧
+    γ₁.length = Γ.length :=
+  by
+  intros 𝓦 γ₀ γ₁ Γ H
+  induction H
+  case nil => simp
+  case cons IH =>
+    constructor
+    . simp; apply IH.left
+    . simp; apply IH.right
+
+lemma log_equiv_env.binds_log_equiv_value :
+  ∀ 𝓦 γ₀ γ₁ Γ x τ,
+    log_equiv_env 𝓦 γ₀ γ₁ Γ →
+    binds x (τ, 𝟚) Γ →
+    log_equiv_value 𝓦 (msubst γ₀ (.fvar x)) (msubst γ₁ (.fvar x)) τ :=
+  by
+  intros 𝓦 γ₀ γ₁ Γ x τ HsemΓ Hbinds
+  induction HsemΓ
+  case nil => nomatch Hbinds
+  case cons v₀ γ₀ v₁ γ₁ τ Γ Hsem_value HsemΓ IH =>
+    have ⟨Hwf₀, Hwf₁⟩ := log_equiv_value.syntactic.wf _ _ _ _ Hsem_value
+    have ⟨HEq₀, HEq₁⟩ := log_equiv_env.length _ _ _ _ HsemΓ
+    simp [HEq₀, HEq₁]
+    by_cases HEqx : Γ.length = x
+    . simp [if_pos HEqx]
+      simp [if_pos HEqx] at Hbinds
+      rw [← Hbinds, identity.msubst, identity.msubst]
+      apply Hsem_value
+      apply Hwf₁.right
+      apply Hwf₀.right
+    . simp [if_neg HEqx]
+      simp [if_neg HEqx] at Hbinds
+      apply IH; apply Hbinds
