CollapsingTowers/TwoLevelMut/LogicalEquiv/Compatibility.lean
@@ -14,8 +14,127 @@ lemma compatibility.fvar :
   simp only [log_equiv_expr]
   intros σ₀ σ₁ Hsem_store
   exists 𝓦, σ₀, σ₁, msubst γ₀ (.fvar x), msubst γ₁ (.fvar x)
-  constructor; admit
+  constructor; apply World.future.refl
   constructor; apply stepn.refl
   constructor; apply stepn.refl
   constructor; apply Hsem_store
-  admit
+  apply log_equiv_env.binds_log_equiv_value _ _ _ _ _ _ HsemΓ Hbinds
+
+-- Γ ⊧ n ≈𝑙𝑜𝑔 n : ℕ
+lemma compatibility.lit :
+  ∀ Γ n,
+    log_equiv Γ (.lit n) (.lit n) .nat :=
+  by
+  intros _ n
+  constructor; apply typing.lit
+  constructor; apply typing.lit
+  intros 𝓦 γ₀ γ₁ HsemΓ
+  simp only [log_equiv_expr]
+  intros σ₀ σ₁ Hsem_store
+  exists 𝓦, σ₀, σ₁, .lit n, .lit n
+  constructor; apply World.future.refl
+  constructor; simp; apply stepn.refl
+  constructor; simp; apply stepn.refl
+  constructor; apply Hsem_store
+  simp
+
+-- Γ ⊧ () ≈𝑙𝑜𝑔 () : unit
+lemma compatibility.unit :
+  ∀ Γ,
+    log_equiv Γ .unit .unit .unit :=
+  by
+  intros n
+  constructor; apply typing.unit
+  constructor; apply typing.unit
+  intros 𝓦 γ₀ γ₁ HsemΓ
+  simp only [log_equiv_expr]
+  intros σ₀ σ₁ Hsem_store
+  exists 𝓦, σ₀, σ₁, .unit, .unit
+  constructor; apply World.future.refl
+  constructor; simp; apply stepn.refl
+  constructor; simp; apply stepn.refl
+  constructor; apply Hsem_store
+  simp
+
+-- Γ ⊧ f₀ ≈𝑙𝑜𝑔 f₁ : τ𝕒 → τ𝕓
+-- Γ ⊧ arg₀ ≈𝑙𝑜𝑔 arg₁ : τ𝕒
+-- —————————————————————————————————
+-- Γ ⊧ f₀ @ arg₀ ≈𝑙𝑜𝑔 f₁ @ arg₁ : τ𝕓
+lemma compatibility.app₁ :
+  ∀ Γ f₀ f₁ arg₀ arg₁ τ𝕒 τ𝕓,
+    log_equiv Γ f₀ f₁ (.arrow τ𝕒 τ𝕓 ⊥) →
+    log_equiv Γ arg₀ arg₁ τ𝕒 →
+    log_equiv Γ (.app₁ f₀ arg₀) (.app₁ f₁ arg₁) τ𝕓 :=
+  by
+  intros Γ f₀ f₁ arg₀ arg₁ τ𝕒 τ𝕓 Hf Harg
+  have ⟨HτFun₀, HτFun₁, Hf⟩ := Hf
+  have ⟨HτArg₀, HτArg₁, Harg⟩ := Harg
+  have Hτ₀ : typing ϵ Γ 𝟚 (.app₁ f₀ arg₀) τ𝕓 ⊥ :=
+    by
+    rw [← Effect.union_pure ⊥, ← Effect.union_pure (⊥ ∪ ⊥)]
+    apply typing.app₁; apply HτFun₀; apply HτArg₀
+  have Hτ₁ : typing ϵ Γ 𝟚 (.app₁ f₁ arg₁) τ𝕓 ⊥ :=
+    by
+    rw [← Effect.union_pure ⊥, ← Effect.union_pure (⊥ ∪ ⊥)]
+    apply typing.app₁; apply HτFun₁; apply HτArg₁
+  constructor; apply Hτ₀
+  constructor; apply Hτ₁
+  intros 𝓦₀ γ₀ γ₁ HsemΓ
+  simp only [log_equiv_expr]
+  intros σ₀ σ₁ Hsem_store
+  --
+  --
+  -- Γ ⊧ f₀ ≈𝑙𝑜𝑔 f₁ : τ𝕒 → τ𝕓
+  -- ————————————————————————————
+  -- 𝓦₁ ⊒ 𝓦₀
+  -- ⟨σ₀, γ₀(f₀)⟩ ⇝* ⟨σ₂, fv₀⟩
+  -- ⟨σ₁, γ₁(f₁)⟩ ⇝* ⟨σ₃, fv₁⟩
+  -- (σ₂, σ₃) : 𝓦₁
+  -- (𝓦₁, fv₀, fv₁) ∈ 𝓥⟦τ𝕒 → τ𝕓⟧
+  simp only [log_equiv_expr] at Hf
+  have ⟨𝓦₁, σ₂, σ₃, fv₀, fv₁, Hfuture₀, HstepFun₀, HstepFun₁, Hsem_store, Hsem_value_fun⟩ := Hf _ _ _ HsemΓ _ _ Hsem_store
+  --
+  --
+  -- Γ ⊧ arg₀ ≈𝑙𝑜𝑔 arg₁ : τ𝕒
+  -- ——————————————————————————————
+  -- 𝓦₂ ⊒ 𝓦₁
+  -- ⟨σ₂, γ₀(arg₀)⟩ ⇝* ⟨σ₄, argv₀⟩
+  -- ⟨σ₃, γ₁(arg₁)⟩ ⇝* ⟨σ₅, argv₁⟩
+  -- (σ₄, σ₅) : 𝓦₂
+  -- (𝓦₂, argv₀, argv₁) ∈ 𝓥⟦τ𝕒⟧
+  simp only [log_equiv_expr] at Harg
+  have ⟨𝓦₂, σ₄, σ₅, argv₀, argv₁, Hfuture₁, HstepArg₀, HstepArg₁, Hsem_store, Hsem_value_arg⟩ := Harg 𝓦₁ _ _ (log_equiv_env.antimono _ _ _ _ _ HsemΓ Hfuture₀) _ _ Hsem_store
+  --
+  --
+  -- (𝓦₁, fv₀, fv₁) ∈ 𝓥⟦τ𝕒 → τ𝕓⟧
+  -- (𝓦₂, argv₀, argv₁) ∈ 𝓥⟦τ𝕒⟧
+  -- ——————————————————————————————————————
+  -- (𝓦₂, fv₀ @ argv₀, fv₁ @ argv₁) ∈ 𝓔⟦τ𝕓⟧
+  have Hsem_expr := log_equiv_value.apply 𝓦₂ _ _ _ _ _ _ (log_equiv_value.antimono _ _ _ _ _ Hsem_value_fun Hfuture₁) Hsem_value_arg
+  --
+  --
+  -- (𝓦₂, fv₀ @ argv₀, fv₁ @ argv₁) ∈ 𝓔⟦τ𝕓⟧
+  -- ——————————————————————————————————————
+  -- ⟨σ₄, fv₀ @ argv₀⟩ ⇝* ⟨σ₆, v₀⟩
+  -- ⟨σ₅, fv₁ @ argv₁⟩ ⇝* ⟨σ₇, v₁⟩
+  simp only [log_equiv_expr] at Hsem_expr
+  have ⟨𝓦₃, σ₆, σ₇, v₀, v₁, Hfuture₂, Hstep₀, Hstep₁, Hsem_store, Hsem_value⟩ := Hsem_expr _ _ Hsem_store
+  exists 𝓦₃, σ₆, σ₇, v₀, v₁
+  constructor
+  . apply World.future.trans _ _ _ Hfuture₂
+    apply World.future.trans _ _ _ Hfuture₁
+    apply Hfuture₀
+  constructor
+  --
+  --
+  -- ⟨σ₀, γ₀(f₀)⟩ ⇝* ⟨σ₂, fv₀⟩
+  -- ⟨σ₂, γ₀(arg₀)⟩ ⇝* ⟨σ₄, argv₀⟩
+  -- ⟨σ₄, fv₀ @ argv₀⟩ ⇝* ⟨σ₆, v₀⟩
+  -- ————————————————————————————————————
+  -- ⟨σ₀, γ₀(f₀) @ γ₀(arg₀)⟩ ⇝* ⟨σ₆, v₀⟩
+  . admit
+  constructor
+  . admit
+  constructor
+  . apply Hsem_store
+  . apply Hsem_value
